ROOT
@@ -354,7 +354,7 @@ session ValidationPaperSnippets in "Papers/Validation" = ConditionalElimination 
     "mathpartir.sty"
 
 
-session CodeGenPaper in "Papers/CodeGen" = Semantics +
+session CodeGenPaper in "Papers/CodeGen" = OptimizationDSL +
   description
     "Snippets of Isabelle theories used for a paper on the code generation facilities"
   options [document = pdf, document_output = "output",
